developmentBS/IdModA_M2_bis.v
@@ -3,8 +3,6 @@ Require Import IdModType.
 Require Import Coq.Lists.List.
 Require Import Coq.Strings.String.
 Require Import Coq.Logic.ProofIrrelevance.
-Require Import ADT.
-Require Import Hardware.
 
 
 Lemma valTyp_irrelevance : forall (T: Type) (p1 p2: ValTyp T), p1 = p2.
@@ -12,8 +10,7 @@ intros.
 eapply proof_irrelevance. 
 Qed.
 
-
-Module IdModA_M2 <: IdModType.
+Module IdModA_M2_b <: IdModType.
  
   Definition Id := string.
 
@@ -24,24 +21,48 @@ Module IdModA_M2 <: IdModType.
   dEq := IdEqDec
   }.
 
+  Inductive page :Type := P (v:nat).
+  Inductive index :Type := I (v:nat).
+  Definition vAddress :Type := list index.
+  Inductive vEntry :Type := VE (a:vAddress).
+  Inductive pEntry :Type := PE (p:page).
+  Inductive sValue : Type := SP:page->sValue 
+                            |SI:index->sValue
+                            |SVA:vAddress->sValue
+                            |SVE:vEntry->sValue
+                            |SPE:pEntry->sValue.
+
+  Definition Vpage (p:page) :nat := match p with |P p' => p' end.
+  Definition Vindex (i:index) :nat := match i with |I i' => i' end.
+  Fixpoint VvAddress (a:vAddress) :(list nat) := 
+        match a with 
+          | nil => nil
+          |cons (I i) ls => cons i (VvAddress ls)
+        end.
+  Definition VvEntry (a:vEntry) :list nat := match a with 
+                    |VE a' => VvAddress a' end.
+  Definition VpEntry (a:pEntry) :nat := match a with | PE a' => Vpage a' end.
+  
+  Definition paddr := prod page index.
+
   Definition IdEq := IdEq2.
- 
+
+  Record state : Type := {
+   currentPartition : page;
+   memory : list (paddr * sValue);
+   partitions : list page
+  }.
+  
   Definition W := state.
 
   Definition Loc_PI := valTyp_irrelevance.
 
-  Lemma Hpx : 0 < nbPage.
-  Proof.
-  specialize nbPageNotZero as H.
-  inversion H.
-  auto.
-  auto.
-  Qed.
-  
+  Definition page0:page := P 0.
 
   Definition BInit := {|
-          currentPartition := {| p:=0 ; Hp := Hpx |} ;
-          memory:= @nil (paddr * value)
+          currentPartition := page0 ;
+          memory:= @nil (paddr * sValue);
+          partitions := @nil page
                       |}.
 
   Instance WP2 : PState W :=
@@ -53,5 +74,5 @@ Module IdModA_M2 <: IdModType.
 
   Definition WP := WP2.
 
-End IdModA_M2.
+End IdModA_M2_b.
 
